Linglib.lean
@@ -237,7 +237,6 @@ import Linglib.Core.Order.IterateFixedPoint
 import Linglib.Core.Order.LeftLinear
 import Linglib.Core.Order.Markedness
 import Linglib.Core.Order.Monotone.Monovary
-import Linglib.Core.Order.Normality
 import Linglib.Core.Order.OfCriteria
 import Linglib.Core.Order.Orthoframe
 import Linglib.Core.Order.Orthoframe.Representation
